$$
\begin{align*}
(k+1)^6&=k^6+6k^5+15k^4+20k^3+15k^2+6k+1\\
(k+1)^6-k^6&=6k^5+15k^4+20k^3+15k^2+6k+1\\
\hline\\
2^6-1^6&=6\cdot1^5+15\cdot1^4+20\cdot1^3+15\cdot1^2+6\cdot1+1\\
3^6-2^6&=6\cdot2^5+15\cdot2^4+20\cdot2^3+15\cdot2^2+6\cdot2+1\\
&\vdots\\
(n+1)^6-n^6&=6n^5+15n^4+20n^3+15n^2+6n+1\\
\hline\\
(n+1)^6-1&=6(1^5+\cdots+n^5)+15(1^4+\cdots+n^4)+20(1^3+\cdots+n^3)+15(1^2+\cdots+n^2)+6(1+\cdots+n)+n\\
(n+1)^6-1&=6\sum^n_{k=1}k^5+15\sum^n_{k=1}k^4+20\sum^n_{k=1}k^3+15\sum^n_{k=1}+6\sum^n_{k=1}k+n\\
6\sum^n_{k=1}k^5&=(n+1)^6-1-15\sum^n_{k=1}k^4-20\sum^n_{k=1}k^3-15\sum^n_{k=1}-6\sum^n_{k=1}k-n\\
6\sum^n_{k=1}k^5&=(n+1)^6-1-n-15\left(\frac{n^5}{5}+\frac{n^4}{2}+\frac{n^3}{3}-\frac{n}{30}\right)-20\left(\frac{n^4}{4}+\frac{n^3}{2}+\frac{n^2}{4}\right)-15\frac{n(n+1)(2n+1)}{6}-6\frac{n(n+1)}{2}\\
6\sum^n_{k=1}k^5&=(n+1)^6-1-n-\frac{15n^5}{5}-\frac{15n^4}{2}-\frac{15n^3}{3}+\frac{15n}{30}-\frac{20n^4}{4}-\frac{20n^3}{2}-\frac{20n^2}{4}-\frac{15n(2n^2+3n+1)}{6}-\frac{6(n^2+n)}{2}\\
6\sum^n_{k=1}k^5&=(n+1)^6-1-n-3n^5-\frac{15n^4}{2}-5n^3+\frac{n}{2}-5n^4-10n^3-5n^2-\frac{30n^3+45n^2+15n}{6}-3n^2-3n\\
6\sum^n_{k=1}k^5&=(n+1)^6-1-4n-3n^5-\frac{15n^4}{2}-15n^3+\frac{n}{2}-5n^4-8n^2-\frac{30n^3+45n^2+15n}{6}\\
6\sum^n_{k=1}k^5&=(n+1)^6-3n^5-5n^4-15n^3-8n^2-4n-1-\frac{15n^4-n}{2}-\frac{30n^3+45n^2+15n}{6}\\
6\sum^n_{k=1}k^5&=(n+1)^6-3n^5-5n^4-15n^3-8n^2-4n-1-\frac{45n^4-3n+30n^3+45n^2+15n}{6}\\
6\sum^n_{k=1}k^5&=(n+1)^6-3n^5-5n^4-15n^3-8n^2-4n-1-\frac{45n^4+30n^3+45n^2+12n}{6}\\
6\sum^n_{k=1}k^5&=(n^6+6n^5+15n^4+20n^3+15n^2+6n+1)-3n^5-5n^4-15n^3-8n^2-4n-1-\frac{45n^4+30n^3+45n^2+12n}{6}\\
6\sum^n_{k=1}k^5&=n^6+3n^5+10n^4+5n^3+7n^2+2n-\frac{45n^4+30n^3+45n^2+12n}{6}\\
6\sum^n_{k=1}k^5&=\frac{6n^6+18n^5+60n^4+30n^3+42n^2+12n}{6}-\frac{45n^4+30n^3+45n^2+12n}{6}\\
6\sum^n_{k=1}k^5&=\frac{6n^6+18n^5+60n^4+30n^3+42n^2+12n-45n^4-30n^3-45n^2-12n}{6}\\
6\sum^n_{k=1}k^5&=\frac{6n^6+18n^5+15n^4-3n^2}{6}\\
6\sum^n_{k=1}k^5&=n^6+3n^5+\frac{5n^4}{2}-\frac{n^2}{2}\\
\sum^n_{k=1}k^5&=\frac{n^6}{6}+\frac{n^5}{2}+\frac{5n^4}{12}-\frac{n^2}{12}\\
\end{align*}
$$